examples/graph/lib/Data/Graph/Inductive/Query/BFS.v
@@ -12,12 +12,12 @@ Require Coq.Program.Wf.
 
 (* Converted imports: *)
 
-Require BinInt.
 Require Coq.Init.Datatypes.
 Require Data.Graph.Inductive.Graph.
 Require Data.Graph.Inductive.Internal.Queue.
 Require Data.Graph.Inductive.Internal.RootPath.
 Require GHC.Base.
+Require GHC.DeferredFix.
 Require GHC.Err.
 Require GHC.List.
 Require GHC.Num.
@@ -49,58 +49,60 @@ Definition outU {a} {b}
     GHC.Base.map Data.Graph.Inductive.Graph.toEdge (Data.Graph.Inductive.Graph.out'
                                                     c).
 
-Program Fixpoint leveln {gr} {a} {b} `{(Data.Graph.Inductive.Graph.Graph gr)}
-                        (arg_0__ : list (Data.Graph.Inductive.Graph.Node * GHC.Num.Int)%type) (arg_1__
-                          : gr a b) {measure (BinInt.Z.abs_nat (Data.Graph.Inductive.Graph.noNodes
-                                                                arg_1__))} : list (Data.Graph.Inductive.Graph.Node *
-                                                                                   GHC.Num.Int)%type
-                   := match arg_0__, arg_1__ with
-                      | nil, _ => nil
-                      | _, g =>
-                          if Bool.Sumbool.sumbool_of_bool (Data.Graph.Inductive.Graph.isEmpty g)
-                          then nil else
-                          match arg_0__, arg_1__ with
-                          | cons (pair v j) vs, g =>
-                              match Data.Graph.Inductive.Graph.match_ v g with
-                              | pair (Some c) g' =>
-                                  cons (pair v j) (leveln (Coq.Init.Datatypes.app vs (suci c (j GHC.Num.+ #1)))
-                                        g')
-                              | pair None g' => leveln vs g'
-                              end
-                          | _, _ => GHC.Err.patternFailure
-                          end
-                      end.
-Admit Obligations.
+Definition leveln {gr} {a} {b} `{(Data.Graph.Inductive.Graph.Graph gr)}
+   : list (Data.Graph.Inductive.Graph.Node * GHC.Num.Int)%type ->
+     gr a b -> list (Data.Graph.Inductive.Graph.Node * GHC.Num.Int)%type :=
+  GHC.DeferredFix.deferredFix2 (fun leveln
+                                (arg_0__ : list (Data.Graph.Inductive.Graph.Node * GHC.Num.Int)%type)
+                                (arg_1__ : gr a b) =>
+                                  match arg_0__, arg_1__ with
+                                  | nil, _ => nil
+                                  | _, g =>
+                                      if Data.Graph.Inductive.Graph.isEmpty g : bool then nil else
+                                      match arg_0__, arg_1__ with
+                                      | cons (pair v j) vs, g =>
+                                          match Data.Graph.Inductive.Graph.match_ v g with
+                                          | pair (Some c) g' =>
+                                              cons (pair v j) (leveln (Coq.Init.Datatypes.app vs (suci c (j GHC.Num.+
+                                                                                                          #1))) g')
+                                          | pair None g' => leveln vs g'
+                                          end
+                                      | _, _ => GHC.Err.patternFailure
+                                      end
+                                  end).
 
 Definition level {gr} {a} {b} `{(Data.Graph.Inductive.Graph.Graph gr)}
    : Data.Graph.Inductive.Graph.Node ->
      gr a b -> list (Data.Graph.Inductive.Graph.Node * GHC.Num.Int)%type :=
   fun v => leveln (cons (pair v #0) nil).
 
-Program Fixpoint lbf {gr} {b} {a} `{(Data.Graph.Inductive.Graph.Graph gr)} (q
-                       : Data.Graph.Inductive.Internal.Queue.Queue (Data.Graph.Inductive.Graph.LPath
-                                                                    b)) (g : gr a b) {measure (BinInt.Z.abs_nat
-                      (Data.Graph.Inductive.Graph.noNodes g))}
-                   : Data.Graph.Inductive.Internal.RootPath.LRTree b
-                   := match Data.Graph.Inductive.Internal.Queue.queueGet q with
-                      | pair (Data.Graph.Inductive.Graph.LP (cons (pair v _) _ as p)) q' =>
-                          if Bool.Sumbool.sumbool_of_bool (orb
-                                                           (Data.Graph.Inductive.Internal.Queue.queueEmpty q)
-                                                           (Data.Graph.Inductive.Graph.isEmpty g))
-                          then nil else
-                          match Data.Graph.Inductive.Graph.match_ v g with
-                          | pair (Some c) g' =>
-                              cons (Data.Graph.Inductive.Graph.LP p) (lbf
-                                    (Data.Graph.Inductive.Internal.Queue.queuePutList (GHC.Base.map (fun v' =>
-                                                                                                       Data.Graph.Inductive.Graph.LP
-                                                                                                       (cons v' p))
-                                                                                       (Data.Graph.Inductive.Graph.lsuc'
-                                                                                        c)) q') g')
-                          | pair None g' => lbf q' g'
-                          end
-                      | _ => GHC.Err.patternFailure
-                      end.
-Admit Obligations.
+Definition lbf {gr} {b} {a} `{(Data.Graph.Inductive.Graph.Graph gr)}
+   : Data.Graph.Inductive.Internal.Queue.Queue (Data.Graph.Inductive.Graph.LPath
+                                                b) ->
+     gr a b -> Data.Graph.Inductive.Internal.RootPath.LRTree b :=
+  GHC.DeferredFix.deferredFix2 (fun lbf
+                                (q
+                                  : Data.Graph.Inductive.Internal.Queue.Queue (Data.Graph.Inductive.Graph.LPath
+                                                                               b))
+                                (g : gr a b) =>
+                                  match Data.Graph.Inductive.Internal.Queue.queueGet q with
+                                  | pair (Data.Graph.Inductive.Graph.LP (cons (pair v _) _ as p)) q' =>
+                                      if orb (Data.Graph.Inductive.Internal.Queue.queueEmpty q)
+                                             (Data.Graph.Inductive.Graph.isEmpty g) : bool
+                                      then nil else
+                                      match Data.Graph.Inductive.Graph.match_ v g with
+                                      | pair (Some c) g' =>
+                                          cons (Data.Graph.Inductive.Graph.LP p) (lbf
+                                                (Data.Graph.Inductive.Internal.Queue.queuePutList (GHC.Base.map
+                                                                                                   (fun v' =>
+                                                                                                      Data.Graph.Inductive.Graph.LP
+                                                                                                      (cons v' p))
+                                                                                                   (Data.Graph.Inductive.Graph.lsuc'
+                                                                                                    c)) q') g')
+                                      | pair None g' => lbf q' g'
+                                      end
+                                  | _ => GHC.Err.patternFailure
+                                  end).
 
 Definition lbft {gr} {a} {b} `{(Data.Graph.Inductive.Graph.Graph gr)}
    : Data.Graph.Inductive.Graph.Node ->
@@ -125,19 +127,20 @@ Definition bfsnInternal {gr} {a} {b} {c} `{(Data.Graph.Inductive.Graph.Graph
    : (Data.Graph.Inductive.Graph.Context a b -> c) ->
      Data.Graph.Inductive.Internal.Queue.Queue Data.Graph.Inductive.Graph.Node ->
      gr a b -> list c :=
-  fix bfsnInternal (f : (Data.Graph.Inductive.Graph.Context a b -> c)) (q
-                     : Data.Graph.Inductive.Internal.Queue.Queue Data.Graph.Inductive.Graph.Node) (g
-                     : gr a b) : list c
-        := let 'pair v q' := Data.Graph.Inductive.Internal.Queue.queueGet q in
-           if orb (Data.Graph.Inductive.Internal.Queue.queueEmpty q)
-                  (Data.Graph.Inductive.Graph.isEmpty g) : bool
-           then nil else
-           match Data.Graph.Inductive.Graph.match_ v g with
-           | pair (Some c) g' =>
-               cons (f c) (bfsnInternal f (Data.Graph.Inductive.Internal.Queue.queuePutList
-                                           (Data.Graph.Inductive.Graph.suc' c) q') g')
-           | pair None g' => bfsnInternal f q' g'
-           end.
+  GHC.DeferredFix.deferredFix3 (fun bfsnInternal
+                                (f : (Data.Graph.Inductive.Graph.Context a b -> c))
+                                (q : Data.Graph.Inductive.Internal.Queue.Queue Data.Graph.Inductive.Graph.Node)
+                                (g : gr a b) =>
+                                  let 'pair v q' := Data.Graph.Inductive.Internal.Queue.queueGet q in
+                                  if orb (Data.Graph.Inductive.Internal.Queue.queueEmpty q)
+                                         (Data.Graph.Inductive.Graph.isEmpty g) : bool
+                                  then nil else
+                                  match Data.Graph.Inductive.Graph.match_ v g with
+                                  | pair (Some c) g' =>
+                                      cons (f c) (bfsnInternal f (Data.Graph.Inductive.Internal.Queue.queuePutList
+                                                                  (Data.Graph.Inductive.Graph.suc' c) q') g')
+                                  | pair None g' => bfsnInternal f q' g'
+                                  end).
 
 Definition bfsnWith {gr} {a} {b} {c} `{(Data.Graph.Inductive.Graph.Graph gr)}
    : (Data.Graph.Inductive.Graph.Context a b -> c) ->
@@ -166,19 +169,19 @@ Definition bfs {gr} {a} {b} `{(Data.Graph.Inductive.Graph.Graph gr)}
 Definition bfenInternal {gr} {a} {b} `{(Data.Graph.Inductive.Graph.Graph gr)}
    : Data.Graph.Inductive.Internal.Queue.Queue Data.Graph.Inductive.Graph.Edge ->
      gr a b -> list Data.Graph.Inductive.Graph.Edge :=
-  fix bfenInternal (q
-                     : Data.Graph.Inductive.Internal.Queue.Queue Data.Graph.Inductive.Graph.Edge) (g
-                     : gr a b) : list Data.Graph.Inductive.Graph.Edge
-        := let 'pair (pair u v) q' := Data.Graph.Inductive.Internal.Queue.queueGet q in
-           if orb (Data.Graph.Inductive.Internal.Queue.queueEmpty q)
-                  (Data.Graph.Inductive.Graph.isEmpty g) : bool
-           then nil else
-           match Data.Graph.Inductive.Graph.match_ v g with
-           | pair (Some c) g' =>
-               cons (pair u v) (bfenInternal (Data.Graph.Inductive.Internal.Queue.queuePutList
-                                              (outU c) q') g')
-           | pair None g' => bfenInternal q' g'
-           end.
+  GHC.DeferredFix.deferredFix2 (fun bfenInternal
+                                (q : Data.Graph.Inductive.Internal.Queue.Queue Data.Graph.Inductive.Graph.Edge)
+                                (g : gr a b) =>
+                                  let 'pair (pair u v) q' := Data.Graph.Inductive.Internal.Queue.queueGet q in
+                                  if orb (Data.Graph.Inductive.Internal.Queue.queueEmpty q)
+                                         (Data.Graph.Inductive.Graph.isEmpty g) : bool
+                                  then nil else
+                                  match Data.Graph.Inductive.Graph.match_ v g with
+                                  | pair (Some c) g' =>
+                                      cons (pair u v) (bfenInternal (Data.Graph.Inductive.Internal.Queue.queuePutList
+                                                                     (outU c) q') g')
+                                  | pair None g' => bfenInternal q' g'
+                                  end).
 
 Definition bfen {gr} {a} {b} `{(Data.Graph.Inductive.Graph.Graph gr)}
    : list Data.Graph.Inductive.Graph.Edge ->
@@ -195,24 +198,26 @@ Definition bfe {gr} {a} {b} `{(Data.Graph.Inductive.Graph.Graph gr)}
 Definition bf {gr} {a} {b} `{(Data.Graph.Inductive.Graph.Graph gr)}
    : Data.Graph.Inductive.Internal.Queue.Queue Data.Graph.Inductive.Graph.Path ->
      gr a b -> Data.Graph.Inductive.Internal.RootPath.RTree :=
-  fix bf (q
-           : Data.Graph.Inductive.Internal.Queue.Queue Data.Graph.Inductive.Graph.Path) (g
-           : gr a b) : Data.Graph.Inductive.Internal.RootPath.RTree
-        := match Data.Graph.Inductive.Internal.Queue.queueGet q with
-           | pair (cons v _ as p) q' =>
-               if orb (Data.Graph.Inductive.Internal.Queue.queueEmpty q)
-                      (Data.Graph.Inductive.Graph.isEmpty g) : bool
-               then nil else
-               match Data.Graph.Inductive.Graph.match_ v g with
-               | pair (Some c) g' =>
-                   cons p (bf (Data.Graph.Inductive.Internal.Queue.queuePutList (GHC.Base.map
-                                                                                 (fun arg_2__ => cons arg_2__ p)
-                                                                                 (Data.Graph.Inductive.Graph.suc' c))
-                               q') g')
-               | pair None g' => bf q' g'
-               end
-           | _ => GHC.Err.patternFailure
-           end.
+  GHC.DeferredFix.deferredFix2 (fun bf
+                                (q : Data.Graph.Inductive.Internal.Queue.Queue Data.Graph.Inductive.Graph.Path)
+                                (g : gr a b) =>
+                                  match Data.Graph.Inductive.Internal.Queue.queueGet q with
+                                  | pair (cons v _ as p) q' =>
+                                      if orb (Data.Graph.Inductive.Internal.Queue.queueEmpty q)
+                                             (Data.Graph.Inductive.Graph.isEmpty g) : bool
+                                      then nil else
+                                      match Data.Graph.Inductive.Graph.match_ v g with
+                                      | pair (Some c) g' =>
+                                          cons p (bf (Data.Graph.Inductive.Internal.Queue.queuePutList (GHC.Base.map
+                                                                                                        (fun arg_2__ =>
+                                                                                                           cons arg_2__
+                                                                                                                p)
+                                                                                                        (Data.Graph.Inductive.Graph.suc'
+                                                                                                         c)) q') g')
+                                      | pair None g' => bf q' g'
+                                      end
+                                  | _ => GHC.Err.patternFailure
+                                  end).
 
 Definition bft {gr} {a} {b} `{(Data.Graph.Inductive.Graph.Graph gr)}
    : Data.Graph.Inductive.Graph.Node ->
@@ -227,13 +232,12 @@ Definition esp {gr} {a} {b} `{(Data.Graph.Inductive.Graph.Graph gr)}
   fun s t => Data.Graph.Inductive.Internal.RootPath.getPath t GHC.Base.∘ bft s.
 
 (* External variables:
-     Bool.Sumbool.sumbool_of_bool None Some bool cons list nil op_zt__ orb pair
-     BinInt.Z.abs_nat Coq.Init.Datatypes.app Data.Graph.Inductive.Graph.Context
-     Data.Graph.Inductive.Graph.Edge Data.Graph.Inductive.Graph.Graph
-     Data.Graph.Inductive.Graph.LP Data.Graph.Inductive.Graph.LPath
-     Data.Graph.Inductive.Graph.Node Data.Graph.Inductive.Graph.Path
-     Data.Graph.Inductive.Graph.isEmpty Data.Graph.Inductive.Graph.lsuc'
-     Data.Graph.Inductive.Graph.match_ Data.Graph.Inductive.Graph.noNodes
+     None Some bool cons list nil op_zt__ orb pair Coq.Init.Datatypes.app
+     Data.Graph.Inductive.Graph.Context Data.Graph.Inductive.Graph.Edge
+     Data.Graph.Inductive.Graph.Graph Data.Graph.Inductive.Graph.LP
+     Data.Graph.Inductive.Graph.LPath Data.Graph.Inductive.Graph.Node
+     Data.Graph.Inductive.Graph.Path Data.Graph.Inductive.Graph.isEmpty
+     Data.Graph.Inductive.Graph.lsuc' Data.Graph.Inductive.Graph.match_
      Data.Graph.Inductive.Graph.node' Data.Graph.Inductive.Graph.out
      Data.Graph.Inductive.Graph.out' Data.Graph.Inductive.Graph.suc'
      Data.Graph.Inductive.Graph.toEdge Data.Graph.Inductive.Internal.Queue.Queue
@@ -246,6 +250,7 @@ Definition esp {gr} {a} {b} `{(Data.Graph.Inductive.Graph.Graph gr)}
      Data.Graph.Inductive.Internal.RootPath.RTree
      Data.Graph.Inductive.Internal.RootPath.getLPath
      Data.Graph.Inductive.Internal.RootPath.getPath GHC.Base.map GHC.Base.op_z2218U__
-     GHC.Err.patternFailure GHC.List.length GHC.List.replicate GHC.List.zip
-     GHC.Num.Int GHC.Num.fromInteger GHC.Num.op_zp__
+     GHC.DeferredFix.deferredFix2 GHC.DeferredFix.deferredFix3 GHC.Err.patternFailure
+     GHC.List.length GHC.List.replicate GHC.List.zip GHC.Num.Int GHC.Num.fromInteger
+     GHC.Num.op_zp__
 *)
